iris_ht_rules.v
@@ -16,7 +16,7 @@ Module Type IRIS_HT_RULES (RL : RA_T) (C : CORE_LANG) (R: IRIS_RES RL C) (WP: WO
 
     Existing Instance LP_isval.
 
-    Implicit Types (P : Props) (i : nat) (safe : bool) (m : mask) (e : expr) (Q : vPred) (r : res).
+    Implicit Types (P : Props) (i : nat) (safe : bool) (m : mask) (e : expr) (Q φ : vPred) (r : res).
 
     (** Ret **)
     Program Definition eqV v : vPred :=
@@ -26,10 +26,10 @@ Module Type IRIS_HT_RULES (RL : RA_T) (C : CORE_LANG) (R: IRIS_RES RL C) (WP: WO
       split; congruence.
     Qed.
 
-    Lemma htRet e (HV : is_value e) safe m :
-      valid (ht safe m ⊤ e (eqV (exist _ e HV))).
+    Lemma wpRet e (HV : is_value e) safe m :
+      valid (wp safe m e (eqV (exist _ e HV))).
     Proof.
-      intros w' nn rr w _ n r' _ _ _; clear w' nn rr.
+      intros w n r'.
       rewrite unfold_wp; intros w'; intros; split; [| split; [| split] ]; intros.
       - exists w' r'; split; [reflexivity | split; [| assumption] ].
         simpl; reflexivity.
@@ -46,34 +46,28 @@ Module Type IRIS_HT_RULES (RL : RA_T) (C : CORE_LANG) (R: IRIS_RES RL C) (WP: WO
     (** Quantification in the logic works over nonexpansive maps, so
         we need to show that plugging the value into the postcondition
         and context is nonexpansive. *)
-    Program Definition plugV safe m Q Q' K :=
-      n[(fun v : value => ht safe m (Q v) (fill K (`v)) Q' )].
+    Program Definition plugCtxWp safe m K φ :=
+      n[(fun v : value => wp safe m (fill K v) φ )].
     Next Obligation.
-      intros v1 v2 EQv; unfold ht; eapply (met_morph_nonexp box).
-      eapply (impl_dist (ComplBI := Props_BI)).
-      - apply Q; assumption.
-      - destruct n as [| n]; [apply dist_bound | simpl in EQv].
-        rewrite EQv; reflexivity.
+      intros v1 v2 EQv.
+      destruct n as [|n]; first by apply: dist_bound.
+      rewrite EQv. reflexivity.
     Qed.
 
-    Lemma htBind P Q R K e safe m :
-      ht safe m P e Q ∧ all (plugV safe m Q R K) ⊑ ht safe m P (fill K e) R.
+    Lemma wpBind φ K e safe m :
+      wp safe m e (plugCtxWp safe m K φ) ⊑ wp safe m (fill K e) φ.
     Proof.
-      intros wz nz rz [He HK] w HSw n r HLe _ HP.
-      specialize (He _ HSw _ _ HLe unit_min HP).
-      rewrite ->HSw, <- HLe in HK; clear wz nz HSw HLe HP.
-      revert e w r He HK; induction n using wf_nat_ind; intros; rename H into IH.
+      intros w n r He.
+      revert e w r He; induction n using wf_nat_ind; intros; rename H into IH.
       rewrite ->unfold_wp in He; rewrite unfold_wp.
       destruct (is_value_dec e) as [HVal | HNVal]; [clear IH |].
       - intros w'; intros; edestruct He as [HV _]; try eassumption; [].
         clear He HE; specialize (HV HVal); destruct HV as [w'' [r' [HSw' [Hφ HE] ] ] ].
         (* Fold the goal back into a wp *)
         setoid_rewrite HSw'.
-        assert (HT : wp safe m (fill K e) R w'' (S k) r');
+        assert (HT : wp safe m (fill K e) φ w'' (S k) r');
           [| rewrite ->unfold_wp in HT; eapply HT; [reflexivity | unfold lt; reflexivity | eassumption | eassumption] ].
-        clear HE; specialize (HK (exist _ e HVal)).
-        do 30 red in HK; unfold proj1_sig in HK.
-        apply HK; [etransitivity; eassumption | apply HLt | apply unit_min | assumption].
+        exact Hφ.
       - intros w'; intros; edestruct He as [_ [HS [HF HS'] ] ]; try eassumption; [].
         split; [intros HVal; contradiction HNVal; assert (HT := fill_value HVal);
                 subst K; rewrite fill_empty in HVal; assumption | split; [| split]; intros].
@@ -83,15 +77,13 @@ Module Type IRIS_HT_RULES (RL : RA_T) (C : CORE_LANG) (R: IRIS_RES RL C) (WP: WO
           edestruct HS as [w'' [r' [HSw' [He HE] ] ] ]; try eassumption; [].
           subst e; clear HStep HS.
           do 2 eexists; split; [eassumption | split; [| eassumption] ].
-          rewrite <- fill_comp. apply IH; try assumption; [].
-          unfold lt in HLt; rewrite <- HSw', <- HSw, Le.le_n_Sn, HLt; apply HK.
+          rewrite <- fill_comp. apply IH; assumption.
         + clear He HS HE; edestruct fork_by_value as [K' EQK]; try eassumption; [].
           subst K0; rewrite <- fill_comp in HDec; apply fill_inj2 in HDec.
           edestruct HF as [w'' [rfk [rret [HSw' [HWR [HWF HE] ] ] ] ] ];
             try eassumption; []; subst e; clear HF.
           do 3 eexists; split; [eassumption | split; [| split; eassumption] ].
-          rewrite <- fill_comp; apply IH; try assumption; [].
-          unfold lt in HLt; rewrite <- HSw', <- HSw, Le.le_n_Sn, HLt; apply HK.
+          rewrite <- fill_comp; apply IH; assumption.
         + clear IH He HS HE HF; specialize (HS' HSafe); clear HSafe.
           destruct HS' as [HV | [HS | HF] ].
           { contradiction. }
@@ -102,6 +94,31 @@ Module Type IRIS_HT_RULES (RL : RA_T) (C : CORE_LANG) (R: IRIS_RES RL C) (WP: WO
     Qed.
 
     (** Consequence **)
+    Lemma wpImpl safe m e φ φ':
+      (□all (lift_bin BI.impl φ φ')) ∧ wp safe m e φ ⊑ wp safe m e φ'.
+    Proof.
+      move=>w n. move: n w e. elim/wf_nat_ind=>n0 IH w0 e r0 [Himpl Hwp].
+      rewrite ->unfold_wp in Hwp. rewrite unfold_wp. intros w1; intros.
+      edestruct Hwp as [Hval [Hstep [Hfork Hsafe]]]; [eassumption|eassumption|eassumption|eassumption|].
+      split; last split; last split.
+      - move=>Hisval. destruct (Hval Hisval) as [w2 [r2 [Hw01 [Hφ Hsat]]]]=>{Hval Hstep Hfork Hsafe}.
+        exists w2 r2. split; first assumption. split; last assumption.
+        eapply (Himpl (exist _ e Hisval)), Hφ.
+        + etransitivity; eassumption.
+        + omega.
+        + by apply: unit_min.
+      - move=>σ' ei ei' K Hfill Hpstep. destruct (Hstep _ _ _ _ Hfill Hpstep) as [w2 [r2 [Hw12 [Hnext Hsat]]]]=>{Hval Hstep Hfork Hsafe}.
+        exists w2 r2. split; first assumption. split; last assumption.
+        eapply IH; last split; last eassumption.
+        + omega.
+        + eapply (propsM (r:=1)); last apply: Himpl; [etransitivity; eassumption|omega|by apply: unit_min].
+      - move=>? ? Heq. destruct (Hfork _ _ Heq) as (w2 & rfk & rret & Hw12 & Hnext1 & Hnext2 & Hsat)=>{Hval Hstep Hfork Hsafe}.
+        exists w2 rfk rret. split; first assumption. split; last (split; assumption).
+        eapply IH; last split; last eassumption.
+        + omega.
+        + eapply (propsM (r:=1)); last apply: Himpl; [etransitivity; eassumption|omega|by apply: unit_min].
+      - assumption.
+    Qed.
 
     (** Much like in the case of the plugging, we need to show that
         the map from a value to a view shift between the applied
@@ -203,9 +220,7 @@ Module Type IRIS_HT_RULES (RL : RA_T) (C : CORE_LANG) (R: IRIS_RES RL C) (WP: WO
     Qed.
 
     (** Framing **)
-
-    (** Helper lemma to weaken the region mask *)
-    Lemma wp_mask_weaken safe m1 m2 e φ (HD : m1 # m2) :
+    Lemma wpFrameMask safe m1 m2 e φ (HD : m1 # m2) :
       wp safe m1 e φ ⊑ wp safe (m1 ∪ m2) e φ.
     Proof.
       intros w n; revert w e φ; induction n using wf_nat_ind; rename H into HInd; intros w e φ r HW.
@@ -233,55 +248,65 @@ Module Type IRIS_HT_RULES (RL : RA_T) (C : CORE_LANG) (R: IRIS_RES RL C) (WP: WO
       - auto.
     Qed.
 
-    Lemma htFrame safe m m' P R e Q (HD : m # m') :
-      ht safe m P e Q ⊑ ht safe (m ∪ m') (P * R) e (lift_bin sc Q (umconst R)).
+    Lemma wpFrameRes safe m e φ R:
+      (wp safe m e φ) * R ⊑ wp safe m e (lift_bin sc φ (umconst R)).
     Proof.
-      intros w n rz He w' HSw n' r HLe _ [r1 [r2 [EQr [HP HLR] ] ] ].
-      specialize (He _ HSw _ _ HLe unit_min HP).
-      clear P w n rz HSw HLe HP; rename w' into w; rename n' into n.
-      apply wp_mask_weaken; [assumption |]; revert e w r1 r EQr HLR He.
-      induction n using wf_nat_ind; intros; rename H into IH.
-      rewrite ->unfold_wp; rewrite ->unfold_wp in He; intros w'; intros.
-      rewrite <- EQr, <- assoc in HE; edestruct He as [HV [HS [HF HS'] ] ]; try eassumption; [].
-      clear He; split; [intros HVal; clear HS HF IH HE | split; [clear HV HF HE | clear HV HS HE; split; [clear HS' | clear HF] ]; intros ].
-      - specialize (HV HVal); destruct HV as [w'' [r1' [HSw' [Hφ HE] ] ] ].
-        rewrite ->assoc in HE. exists w'' (r1' · r2).
-        split; [eassumption | split; [| eassumption ] ].
-        exists r1' r2; split; [reflexivity | split; [assumption |] ].
-        unfold lt in HLt; rewrite ->HLt, <- HSw', <- HSw; apply HLR.
-      - edestruct HS as [w'' [r1' [HSw' [He HE] ] ] ]; try eassumption; []; clear HS.
-        destruct k as [| k]; [exists w' r1'; split; [reflexivity | split; [apply wpO | exact I] ] |].
-        rewrite ->assoc in HE. exists w'' (r1' · r2).
-        split; [eassumption | split; [| eassumption] ].
-        eapply IH; try eassumption; [ reflexivity |].
-        unfold lt in HLt; rewrite ->Le.le_n_Sn, HLt, <- HSw', <- HSw; apply HLR.
-      - specialize (HF _ _ HDec); destruct HF as [w'' [rfk [rret [HSw' [HWF [HWR HE] ] ] ] ] ].
-        destruct k as [| k]; [exists w' rfk rret; split; [reflexivity | split; [apply wpO | split; [apply wpO | exact I] ] ] |].
-        rewrite ->assoc, <- (assoc rfk) in HE.
-        exists w''. exists rfk (rret · r2).
-        split; [eassumption | split; [| split; eassumption] ].
-        eapply IH; try eassumption; [ reflexivity |].
-        unfold lt in HLt; rewrite ->Le.le_n_Sn, HLt, <- HSw', <- HSw; apply HLR.
+      move=> w n; revert w e φ R; induction n using wf_nat_ind; rename H into HInd; intros w e φ R r HW.
+      rewrite unfold_wp; rewrite ->unfold_wp in HW; intros w'; intros.
+      destruct HW as [r1 [r2 [EQr [Hwp HR]]]]. pose (rf' := r2 · rf).
+      edestruct Hwp with (rf:=rf') as [HV [HS [HF HS'] ] ]; try eassumption.
+      { eapply wsat_equiv, HE; last reflexivity.
+        - clear; intros j; unfold mcup; tauto.
+        - unfold rf'. rewrite -EQr assoc. reflexivity. }
+      subst rf'.
+      clear Hwp HE; split; [intros HVal; clear HS HF HInd | split; [intros; clear HV HF | split; [intros; clear HV HS | intros; clear HV HS HF] ] ].
+      - specialize (HV HVal); destruct HV as [w'' [r' [HSW [Hφ HE] ] ] ].
+        do 2 eexists; split; [eassumption | split ].
+        + exists r' r2. split; first reflexivity.
+          split; first assumption.
+          eapply propsMWN, HR; [etransitivity; eassumption|omega].
+        + eapply wsat_equiv, HE; try reflexivity.
+          * rewrite assoc. reflexivity.
+      - edestruct HS as [w'' [r' [HSW [HW HE] ] ] ]; try eassumption; []; clear HS.
+        do 2 eexists; split; [eassumption | split ].
+        + eapply HInd; [omega|].
+          exists r' r2. split; first reflexivity.
+          split; first by eapply HW.
+          eapply propsMWN, HR; [etransitivity; eassumption|omega].
+        + eapply wsat_equiv, HE; try reflexivity.
+          * rewrite assoc. reflexivity.
+      - destruct (HF _ _ HDec) as [w'' [rfk [rret [HSW [HWR [HWF HE] ] ] ] ] ]; clear HF.
+        do 3 eexists; split; [eassumption |].
+        split; last split.
+        + eapply HInd; first omega.
+          exists rret r2. split; first reflexivity.
+          split; first assumption.
+          eapply propsMWN, HR; [etransitivity; eassumption|omega].
+        + assert (Heq: umconst ⊤ == lift_bin sc (umconst ⊤) (umconst ⊤)).
+          { clear. move=>v. change ((⊤:Props) == ⊤*⊤). rewrite sc_top_unit. reflexivity. }
+          rewrite Heq=>{Heq}. eapply HInd; first omega.
+          exists rfk ra_unit. split; first reflexivity.
+          split; first assumption.
+          exact I.
+        + eapply wsat_equiv, HE; try reflexivity.
+          * rewrite ->ra_op_unit2, !assoc. reflexivity.
       - auto.
     Qed.
 
-    Lemma htAFrame safe m m' P R e Q
-          (HD  : m # m')
+    Lemma wpAFrameRes safe m R e φ
           (HAt : atomic e) :
-      ht safe m P e Q ⊑ ht safe (m ∪ m') (P * ▹R) e (lift_bin sc Q (umconst R)).
+      (wp safe m e φ) * ▹R ⊑ wp safe m e (lift_bin sc φ (umconst R)).
     Proof.
-      intros w n rz He w' HSw n' r HLe _ [r1 [r2 [EQr [HP HLR] ] ] ].
-      specialize (He _ HSw _ _ HLe unit_min HP).
-      clear rz n HLe; apply wp_mask_weaken; [assumption |]; rewrite ->unfold_wp.
-      clear w HSw; rename n' into n; rename w' into w; intros w'; intros.
+      intros w n r [r1 [r2 [EQr [Hwp HLR]]]].
+      rewrite->unfold_wp; intros w'; intros.
       split; [intros; exfalso | split; intros; [| split; intros; [exfalso| ] ] ].
       - contradiction (atomic_not_value e).
       - destruct k as [| k];
         [exists w' r; split; [reflexivity | split; [apply wpO | exact I] ] |].
-        rewrite ->unfold_wp in He; rewrite <- EQr, <- assoc in HE.
-        edestruct He as [_ [HeS _] ]; try eassumption; [].
+        rewrite ->unfold_wp in Hwp. rewrite <- EQr, <- assoc in HE.
+        edestruct Hwp as [_ [HeS _] ]; try eassumption; [].
         edestruct HeS as [w'' [r1' [HSw' [He' HE'] ] ] ]; try eassumption; [].
-        clear HE He HeS; rewrite ->assoc in HE'.
+        clear HE Hwp HeS; rewrite ->assoc in HE'.
         exists w'' (r1' · r2).
         split; [eassumption | split; [| eassumption] ].
         assert (HNV : ~ is_value ei)
@@ -306,28 +331,26 @@ Module Type IRIS_HT_RULES (RL : RA_T) (C : CORE_LANG) (R: IRIS_RES RL C) (WP: WO
           contradiction (fork_not_value e').
         + unfold safeExpr. now auto.
       - subst; eapply fork_not_atomic; eassumption.
-      - rewrite <- EQr, <- assoc in HE; rewrite ->unfold_wp in He.
-        specialize (He w' k (r2 · rf) mf σ HSw HLt HD0 HE); clear HE.
-        destruct He as [_ [_ [_ HS'] ] ]; auto.
+      - rewrite <- EQr, <- assoc in HE; rewrite ->unfold_wp in Hwp.
+        specialize (Hwp w' k (r2 · rf) mf σ HSw HLt HD HE); clear HE.
+        destruct Hwp as [_ [_ [_ HS'] ] ]; auto.
     Qed.
 
     (** Fork **)
-    Lemma htFork safe m P R e :
-      ht safe m P e (umconst ⊤) ⊑ ht safe m (▹P * ▹R) (fork e) (lift_bin sc (eqV (exist _ fork_ret fork_ret_is_value)) (umconst R)).
+    Lemma wpFork safe m R e :
+      ▹wp safe m e (umconst ⊤) * ▹R ⊑ wp safe m (fork e) (lift_bin sc (eqV (exist _ fork_ret fork_ret_is_value)) (umconst R)).
     Proof.
-      intros w n rz He w' HSw n' r HLe _ [r1 [r2 [EQr [HP HLR] ] ] ].
-      destruct n' as [| n']; [apply wpO |].
-      simpl in HP; specialize (He _ HSw _ _ (Le.le_Sn_le _ _ HLe) unit_min HP).
-      clear rz n HLe; rewrite ->unfold_wp.
-      clear w HSw HP; rename n' into n; rename w' into w; intros w'; intros.
+      intros w n r [r1 [r2 [EQr [Hwp HLR] ] ] ].
+      destruct n as [| n]; [apply wpO |].
+      rewrite ->unfold_wp; intros w'; intros.
       split; [intros; contradiction (fork_not_value e) | split; intros; [exfalso | split; intros ] ].
       - assert (HT := fill_fork HDec); subst K; rewrite ->fill_empty in HDec; subst.
         eapply fork_stuck with (K := ε); [| repeat eexists; eassumption ]; reflexivity.
       - assert (HT := fill_fork HDec); subst K; rewrite ->fill_empty in HDec.
         apply fork_inj in HDec; subst e'; rewrite <- EQr in HE.
-        unfold lt in HLt; rewrite <- (le_S_n _ _ HLt), HSw in He.
+        unfold lt in HLt. simpl in Hwp.
         simpl in HLR; rewrite <- Le.le_n_Sn in HE.
-        do 3 eexists; split; [reflexivity | split; [| split; eassumption] ].
+        do 3 eexists; split; [reflexivity | split; [| split; [eapply propsMWN, Hwp;[eassumption|omega]| eassumption]]].
         rewrite ->fill_empty; rewrite ->unfold_wp; rewrite <- (le_S_n _ _ HLt), HSw in HLR.
         clear - HLR; intros w''; intros; split; [intros | split; intros; [exfalso | split; intros; [exfalso |] ] ].
         + do 2 eexists; split; [reflexivity | split; [| eassumption] ].
@@ -342,18 +365,16 @@ Module Type IRIS_HT_RULES (RL : RA_T) (C : CORE_LANG) (R: IRIS_RES RL C) (WP: WO
       - right; right; exists e empty_ctx; rewrite ->fill_empty; reflexivity.
     Qed.
 
-    Lemma htUnsafe {m P e Q} : ht true m P e Q ⊑ ht false m P e Q.
+    Lemma wpUnsafe {m e φ} : wp true m e φ ⊑ wp false m e φ.
     Proof.
-      move=> wz nz rz He w HSw n r HLe _ HP.
-      move: {He P wz nz rz HSw HLe HP} (He _ HSw _ _ HLe unit_min HP).
-      move: n e Q w r; elim/wf_nat_ind; move=> n IH e Q w r He.
+      move=> w n. move: n w e φ; elim/wf_nat_ind. move=> n IH w e φ r He.
       rewrite unfold_wp; move=> w' k rf mf σ HSw HLt HD HW.
       move/(_ _ HLt): IH => IH.
       move/unfold_wp/(_ _ _ _ _ _ HSw HLt HD HW): He => [HV [HS [HF _] ] ] {HSw HLt HD HW}.
       split; [done | clear HV; split; [clear HF | split; [clear HS | done] ] ].
       - move=> σ' ei ei' K HK Hs.
         move/(_ _ _ _ _ HK Hs): HS => [w'' [r' [HSw' [He' Hw'] ] ] ] {Hs HK}.
-        exists w'' r'. split; [done | split; [exact: IH | done] ].
+        exists w'' r'. split; [done | split; [ by apply:IH | done] ].
       - move=> e' K HK.
         move/(_ _ _ HK): HF => [w'' [rfk [rret [HSw' [Hk [He' HW']]]]]] {HK}.
         exists w'' rfk rret. split; [done | split; [exact: IH | split; [exact: IH | done] ] ].
